bedrock2/src/bedrock2/WordNotations.v
@@ -1,14 +1,14 @@
-Require Import coqutil.Word.Interface.
+Require Import coqutil.Word.Bitwidth.
 
 Declare Scope word_scope.
 
-Infix "^+" := word.add  (at level 50, left associativity) : word_scope.
-Infix "^-" := word.sub  (at level 50, left associativity) : word_scope.
-Infix "^*" := word.mul  (at level 40, left associativity) : word_scope.
-Infix "^<<" := word.slu  (at level 37, left associativity) : word_scope.
-Infix "^>>" := word.sru  (at level 37, left associativity) : word_scope.
+Infix "^+" := Zmod.add  (at level 50, left associativity) : word_scope.
+Infix "^-" := Zmod.sub  (at level 50, left associativity) : word_scope.
+Infix "^*" := Zmod.mul  (at level 40, left associativity) : word_scope.
+Infix "^<<" := Zmod.slu  (at level 37, left associativity) : word_scope.
+Infix "^>>" := Zmod.sru  (at level 37, left associativity) : word_scope.
 
 (* squeeze a Z into a word (beat it with a / to make it smaller) *)
-Notation "/[ x ]" := (word.of_Z x) (format "/[ x ]") : word_scope.
+Notation "/[ x ]" := (Zmod.of_Z _ x) (format "/[ x ]") : word_scope.
 (* \ is the open (removed) lid of the modulo box imposed by words, *)
-Notation "\[ x ]" := (word.unsigned x) (format "\[ x ]") : word_scope.
+Notation "\[ x ]" := (Zmod.unsigned x) (format "\[ x ]") : word_scope.
